docs/formal/python_semantic/Map.v
@@ -1,334 +1,83 @@
-Require Import Arith Ascii String List Sorted.
-Import ListNotations.
-Require Import Pyre.Lib.List Pyre.Lib.String.
+From Coq Require Import Structures.OrderedTypeEx.
+From Coq Require Import FMapList.
+From Coq Require Import String.
+From Pyre Require Typ Statement.
 
-(** In this module, we define the main <<State>> structure of our judgements.
-The underlying structure is a <<Map>> indexed by <<string>>s. They are
-implemented using lists of "key/value" pairs, strictly (no duplicated entries)
-sorted by keys. *)
+Module SMap := FMapList.Make(String_as_OT).
 
-(* Some helper definitions to deal encapsulate/project the order on string to
-order of pairs of (string/anything). *)
-Section SortedListHelpers.
-Variable A: Type.
+(** * Information about function definitions
 
-(* Pair comparison by only using the first member *)
-Definition pair_lt (elt0 elt1: string * A) : Prop :=
-  String.lt (fst elt0) (fst elt1)
-.
-
-(* begin hide *)
-Lemma HdRel_pair_lt_right: forall l key value0 value1,
-  HdRel pair_lt (key, value0) l -> HdRel pair_lt (key, value1) l.
-Proof.
-intros [ | hd tl] key v0 v1 h; simpl in *; [ now constructor | ].
-apply HdRel_inv in h; constructor.
-now unfold pair_lt in *.
-Qed.
-
-Lemma pair_lt_trans: forall (x y z: string * A),
-  pair_lt x y -> pair_lt y z -> pair_lt x z.
-Proof.
-intros [x0 x1] [y0 y1] [z0 z1]; intros h0 h1; simpl in *.
-now apply String.lt_trans with (y := y0).
-Qed.
-
-Lemma Forall_pair_lt: forall key1 value1 key2 value2,
-  pair_lt (key1, value1) (key2, value2) ->
-  forall l, Forall (pair_lt (key2, value2)) l ->
-  Forall (pair_lt (key1, value1)) l.
-Proof.
-intros key1 value1 key2 value2 hp.
-induction l as [ | [k v] l hi]; intros hf; simpl in *; [ now constructor | ].
-constructor.
-- eapply pair_lt_trans; [now apply hp| ].
-  now apply Forall_inv in hf.
-- apply hi.
-  now apply Forall_inv_tail in hf.
-Qed.
-(* end hide *)
-End SortedListHelpers.
-
-(** * Map
-
-A <<Map>> is a stricly sorted list of key/value pairs which helps keeping
-track of types / values in the rest of the developlment. *)
-Section Map.
-
-(* Generic type of values *)
-Context {A: Set}.
-
-(** Generic definition of partial maps from identifiers to some type A
-    encoded as sorted lists of pairs *)
-Record Map : Set := mkMap {
-  data :> list (string * A); (* Maps can be coerced to their data field *)
-  correct : @Sorted _ (pair_lt _) data
+We store in here all relevant information about known functions:
+- their <<name>>.
+- their signature, as a list of <<parameters>> and a <<return annotation>>.
+- the actual <<body>> statement of the function.
+*)
+Record func : Set := mkFun {
+    (* TODO(T53097965): support dotted access for methods *)
+    name: string;
+    (* TODO(T53097965): support more parameter kinds *)
+    parameters: list (string * Typ.t);
+    (* decorators: Expression.t list; *)
+    return_annotation: Typ.t; (* no option, set to TNone if need be *)
+    (* async: bool; *)
+    (* parent: Reference.t option; (1* The class owning the method. *1) *)
+    body: Statement.t;
 }.
 
-(** The empty map *)
-Definition empty: Map := mkMap nil (Sorted_nil _).
-
-(** Reading from a map, might return None if the key is not present *)
-Fixpoint get_map_ (map: list (string * A)) id : option A :=
-  match map with 
-  | nil => None
-  | (key, value) :: map =>
-      if (id =? key)%string
-      then Some value
-      else get_map_ map id
-end.
-
-(* wrapper around get_map_ *)
-Definition get_map (map: Map) key : option A := get_map_ map key.
-
-(** Updating a binding in a map: since we always keep our lists sorted,
-    we proceed by insertion sort, overriding the existing value if the 
-    key was already in use. *)
-Fixpoint insert_sorted (key: string) (value: A)
-  (l: list (string * A)) : list (string * A) :=
-  match l with
-  | [] => [(key, value)]
-  | (key', value') :: l' =>
-      if (key =? key')%string
-      then (key, value) :: l'
-      else if String.ltb key key'
-           then (key, value) :: l
-           else (key', value') :: insert_sorted key value l'
-  end.
-
-(* begin hide *)
-Lemma insert_sorted_hdrel: forall l key value,
-  HdRel (pair_lt _) (key, value) l ->
-  forall key' value',
-  String.lt key key' ->
-  HdRel (pair_lt _) (key, value) (insert_sorted key' value' l).
-Proof.
-induction l as [ | [k v] data hi]; intros key value hhd key' value' hlt;
-    simpl in *; [now constructor | ].
-apply HdRel_inv in hhd; unfold pair_lt in hhd; simpl in hhd.
-case_eq (String.eqb key' k); intro heq.
-- now constructor.
-- case_eq (ltb key' k); intro hk;  now constructor.
-Qed.
-
-Lemma insert_sorted_sorts: forall l, Sorted (pair_lt _) l ->
-  forall key value, Sorted (pair_lt _) (insert_sorted key value l).
-Proof.
-induction l as [ | [key value] data hi]; intros hsort key' value';
-    simpl in *; [ now repeat constructor | ].
-case_eq (String.eqb key' key); intro heq.
-- apply Sorted_inv in hsort as [ h0 h1].
-  constructor; [ assumption | ].
-  apply String.eqb_eq in heq; subst.
-  now apply HdRel_pair_lt_right with (value0 := value).
-- case_eq (ltb key' key); intro hkeys.
-  + constructor; [ assumption | ].
-    apply String.ltb_lt in hkeys.
-    now constructor; unfold pair_lt; simpl.
-  + apply Sorted_inv in hsort as [ h0 h1].
-    constructor; [ now apply hi | ].
-    apply insert_sorted_hdrel;[ assumption | ].
-    apply String.eqb_neq in heq.
-    apply String.lt_ge in hkeys as [ h | h ]; [ now apply String.ltb_lt | ].
-    now elim heq.
-Qed.
-(* end hide *)
-
-(** Set a <<key>> to some <<value>> in a <<Map>>, overriding the existing
-    value if the <<key>> was already in use. *)
-Definition set_map (map: Map) key (value: A) : Map := 
-  let new_data := insert_sorted key value map in
-  mkMap new_data (insert_sorted_sorts map (correct map) key value).
-
-(** Removing a key/value pair in a sorted list, based on the key.
-    Since we are stricly sorted, the first one (if any) is the only one *)
-Fixpoint remove_sorted (l: list (string * A)) id : list (string * A) :=
-  match l with 
-  | nil => nil
-  | (key, value) :: l =>
-      if (id =? key)%string
-      then l
-      else (key, value) :: remove_sorted l id
-end.
-
-(* begin hide *)
-Lemma remove_sorted_forall: forall l key value,
-  Forall (pair_lt _ (key, value)) l ->
-  forall key',
-  Forall (pair_lt _ (key, value)) (remove_sorted l key').
-Proof.
-induction l as [ | [key value] l hi]; intros k v hf key'; simpl in *;
-    [now constructor | ].
-case_eq (String.eqb key' key); intro heq; [ now apply Forall_inv_tail in hf | ].
-constructor; [now apply Forall_inv in hf | ].
-apply hi.
-now apply Forall_inv_tail in hf.
-Qed.
-
-Lemma remove_sorted_strongly_sorted: forall l,
-  StronglySorted (pair_lt _) l -> forall key,
-  StronglySorted (pair_lt _) (remove_sorted l key).
-Proof.
-induction 1 as [ | [key value] data hdata hi hforall ]; intros key';
-    simpl in *; [ now constructor | ].
-case_eq (String.eqb key' key); intro hk; [ assumption | ].
-constructor; [now apply hi | ].
-now apply remove_sorted_forall.
-Qed.
-
-Lemma remove_sorted_sorts: forall l, Sorted (pair_lt _) l ->
-  forall key, Sorted (pair_lt _) (remove_sorted l key).
-Proof.
-intros l hs k.
-apply StronglySorted_Sorted.
-apply remove_sorted_strongly_sorted.
-apply Sorted_StronglySorted; [| assumption].
-intros x y z.
-now apply pair_lt_trans.
-Qed.
-(* end hide *)
-
-(** Remove an entry from a map. Once this function terminates, the <<key>>
-  is no longer mapped to anything in the map. *)
-Definition unset_map (map: Map) key : Map :=
-  let new_data := remove_sorted (data map) key in 
-  mkMap new_data (remove_sorted_sorts (data map) (correct map) key).
-
-(* If a <<key>> is less that all the keys in a list, then getting <<key>>
-   from the list will return nothing. *)
-Lemma get_lt_none: forall l key value, Forall (pair_lt _ (key, value)) l ->
-  get_map_ l key = None.
-Proof.
-induction l as [ | [k v] l hi]; intros key value hf; simpl in *; [reflexivity | ].
-case_eq (String.eqb key k); intro hk.
-- apply Forall_inv in hf.
-  unfold pair_lt in hf; simpl in hf.
-  apply String.lt_not_eq in hf.
-  elim hf.
-  now apply String.eqb_eq.
-- apply Forall_inv_tail in hf.
-  now apply hi in hf.
-Qed.
-
-Lemma get_set_map: forall map x y a,
-  get_map (set_map map x a) y =
-  if  (y =? x)%string then Some a else get_map map y.
-Proof.
-intros [l hs] x y a; unfold set_map, get_map; simpl.
-induction l as [ | [k v] l hi]; simpl in *; [reflexivity | ].
-case_eq (String.eqb x k); intro hk; simpl.
-- case_eq (String.eqb y x); intro hyx; rewrite hyx in *; [reflexivity | ].
-  apply String.eqb_eq in hk as ->.
-  now rewrite hyx.
-- apply Sorted_inv in hs as [hs hhd].
-  case_eq (ltb x k); intro hlt; simpl.
-  + now case_eq (String.eqb y x); intro hyx; rewrite hyx in *.
-  + case_eq (String.eqb y x); intro hyx; rewrite hyx in *.
-    * apply String.eqb_eq in hyx; subst.
-      rewrite hk.
-      now apply hi.
-    * case_eq (String.eqb y k); intro hyk; [reflexivity | ].
-      now apply hi.
-Qed.
-
-Lemma get_unset_map:
-  forall map x z,
-  get_map (unset_map map x) z =
-  if (z =? x)%string then None else get_map map z.
-Proof.
-unfold unset_map, get_map; simpl.
-intros [l hs] x z.
-induction l as [ | [k v] l hi]; simpl in *; [ now destruct String.eqb | ].
-apply Sorted_inv in hs as [hs hhd].
-case_eq (z =? x)%string; intro hzx; rewrite hzx in hi.
-- case_eq (x =? k)%string; intro hxk; simpl.
-  + apply String.eqb_eq in hzx.
-    apply String.eqb_eq in hxk; subst.
-    apply get_lt_none with (value := v).
-    now apply HdRel_Forall; [ now apply pair_lt_trans | | ].
-  + apply String.eqb_eq in hzx; subst.
-    rewrite hxk.
-    now apply hi.
-- case_eq (x =? k)%string; intro hxk; simpl.
-  + apply String.eqb_eq in hxk; subst.
-    now rewrite hzx.
-  + case_eq (z =? k)%string; intro hzk; simpl; [ reflexivity | ].
-    now apply hi.
-Qed.
-
-(** Intermediate "state", which will be used to track types or values
-associated with identifiers *)
-Record RawState0: Set := mkRawState0 {
-    local: Map;
+(** Global state for the statement operational semantic. It is made of
+the state for expression evaluation, along with information about know
+functions. *)
+Record State {A: Set} := mkState {
+  RawState :> SMap.t A;
+  FuncState : SMap.t func 
 }.
 
-(* Wrappers around their _map counter-part *)
-Definition Empty0 : RawState0 := mkRawState0 empty.
+Definition set {A: Set} (state: @State A) (id: string) (v: A) :=
+  mkState _ (SMap.add id v state) (FuncState state).
 
-Definition get0 s k := get_map (local s) k.
+Definition remove {A: Set} (state : @State A) (id: string) : @State A :=
+  mkState _ (SMap.remove id state) (FuncState state).
 
-Definition set0 st k (v: A) :=
-    mkRawState0 (set_map (local st) k v).
 
-Definition unset0 st k :=
-    mkRawState0 (unset_map (local st) k).
+Definition get_info {A: Set} (state: @State A) (fun_name: string) : option func :=
+  SMap.find fun_name (FuncState state).
 
-Lemma get0_set0: forall s x y a,
-  get0 (set0 s x a) y =
-  if (y =? x)%string then Some a else get0 s y.
+From Coq Require Import FMapFacts.
+
+Module SMapFacts := WFacts (SMap).
+
+Lemma find_add_smap: forall {A: Set} (state : SMap.t A) (x y: string) (v : A),
+  SMap.find y (SMap.add x v state) =
+  if (y =? x)%string then Some v else SMap.find y state.
 Proof.
-intros s x y a; unfold set0, get0; simpl.
-now rewrite get_set_map.
+intros A state x y v.
+case_eq (String.eqb y x); intro hyx.
+- apply SMapFacts.add_eq_o.
+  apply String.eqb_eq in hyx; rewrite hyx; reflexivity.
+- apply SMapFacts.add_neq_o.
+  apply String.eqb_neq in hyx.
+  firstorder.
 Qed.
 
-Lemma get0_unset0:
-  forall s x z,
-  get0 (unset0 s x) z =
-  if (z =? x)%string then None else get0 s z.
+Lemma find_add: forall {A: Set} (state : @State A) (x y: string) (v : A),
+  SMap.find y (set state x v) =
+  if (y =? x)%string then Some v else SMap.find y state.
 Proof.
-intros s x z; unfold unset0, get0; simpl.
-now rewrite get_unset_map.
+intros A state x y v.
+unfold set; simpl.
+rewrite find_add_smap.
+reflexivity.
 Qed.
 
-End Map.
-
-Section RawState.
-Context {A B: Set}.
-
-(** Main "state", which stores a <<RawState0>> plus additional information
-  (like a list of the already checked/defined functions.
-  We implicitely coerce <<RawState>> to their underlying <<RawState0>>. *)
-Record RawState : Set := mkRawState {
-    state :> @RawState0 A;
-    info : @Map B;
-}.
-
-Definition Empty (info: @Map B) : RawState := mkRawState Empty0 info.
-
-Definition get (s: RawState) id := get0 (state s) id.
-Definition set (s: RawState) id v :=
-    mkRawState (set0 s id v) (info s).
-Definition unset (s: RawState) id :=
-    mkRawState (unset0 s id) (info s).
-
-Definition get_info (s: RawState) f := get_map (info s) f.
-
-Lemma get_set: forall s x y a,
-  get (set s x a) y =
-  if  (y =? x)%string then Some a else get s y.
+Lemma find_remove_smap: forall {A : Set} (state: @SMap.t A) (x z: string),
+  SMap.find z (SMap.remove x state) =
+  if (z =? x)%string then None else SMap.find z state.
 Proof.
-intros [s ?] x y a; simpl.
-unfold set, get; simpl state.
-now rewrite get0_set0.
+intros A state x z.
+case_eq (String.eqb z x); intro hzx.
+- apply SMapFacts.remove_eq_o.
+  apply String.eqb_eq in hzx; rewrite hzx; reflexivity.
+- apply SMapFacts.remove_neq_o.
+  apply String.eqb_neq in hzx.
+  firstorder.
 Qed.
-
-Lemma get_unset:
-  forall s x z,
-  get (unset s x) z =
-  if (z =? x)%string then None else get s z.
-Proof.
-intros s x z; unfold unset, get; simpl.
-now rewrite get0_unset0.
-Qed.
-
-End RawState.
